progress on LightFilter

examples/sbf/LightFilter.v
@@ -1,9 +1,9 @@
 Require Import Coq.ZArith.BinInt.
 Require Import Coq.Program.Program.
 Require Poulet4.Utils.Utils.
+Require Import ProD3.core.Coqlib.
 Require Import ProD3.examples.sbf.Utils.
 Require Import ProD3.examples.sbf.AbsFilter.
-Require Import ProD3.core.Coqlib.
 Require Import Hammer.Plugin.Hammer.
 Import ListNotations.
 Open Scope Z_scope.
@@ -12,60 +12,152 @@ Open Scope program_scope.
 Section LightFilter.
 
 Context {header_type : Set}.
+Context (num_frames num_rows num_slots frame_time : Z).
+Hypothesis H_num_slots : 0 < num_slots.
+Hypothesis H_num_rows : 0 < num_rows.
+Context (hashes : list (header_type -> Z)).
+Hypothesis H_Zlength_hashes : Zlength hashes = num_rows.
+Hypothesis H_hashes : Forall (fun hash => forall h, 0 <= hash h < num_slots) hashes.
 
-Axiom filter_base : Type.
-Definition filter := option filter_base.
+Context (tick_time : Z).
+Hypothesis (H_tick_time : 0 < tick_time).
+Context (round_time : Z -> Z).
 
-(* The time of guaranteed query, e.g. 60s. *)
-Axiom T : Z.
-(* The maximum time interval between consecutive packets, e.g. 100us. *)
-Axiom Tc : Z.
+Hypothesis (H_frame_time : 0 < frame_time).
+Hypothesis (H_tick_time_div : (tick_time * 2 | frame_time)).
 
-Axiom filter_insert : filter -> (Z * header_type) -> filter.
-Axiom filter_query : filter -> (Z * header_type) -> option bool.
-Axiom filter_clear : filter -> Z -> filter.
-Axiom filter_empty : filter.
+Definition filter := option (@filter header_type).
 
-Lemma filter_query_clear : forall f t t' h b,
-  isSome (filter_clear f t) ->
-  filter_query f (t', h) = Some b ->
-  filter_query (filter_clear f t) (t', h) = Some b.
+Notation abs_insert := (@filter_insert header_type num_frames num_slots frame_time tick_time).
+Notation abs_query := (@filter_query header_type num_frames num_slots frame_time hashes tick_time).
+Notation abs_clear := (@filter_clear header_type num_frames num_slots frame_time tick_time).
+
+(* The time of guaranteed query, e.g. 59s. *)
+Definition T := frame_time * (num_frames - 2).
+
+(* The maximum time interval between consecutive packets, e.g. 112us. *)
+Definition Tc := (frame_time - 1) / num_slots + 1.
+
+(* This should be provable *)
+Axiom Tc_mul_num_slots_ge_frame_time : Tc * num_slots >= frame_time.
+(* This seems NOT provable. *)
+Axiom Tc_le_tick_time : Tc <= tick_time.
+Lemma Tc_le_frame_time : Tc <= frame_time.
 Admitted.
 
-Lemma filter_query_insert_same : forall f t t' h,
-  0 <= t' - t < T ->
-  isSome f ->
+Definition filter_insert (f : filter) (th : Z * header_type) : filter :=
+  match f with
+  | Some f => abs_insert f th
+  | None => None
+  end.
+
+(* TODO this is incorrect. *)
+Definition filter_query (f : filter) (th : Z * header_type) : option bool :=
+  match f with
+  | Some f =>
+      option_map snd (abs_query f th)
+  | None => None
+  end.
+
+Definition filter_clear (f : filter) (t : Z) : filter :=
+  match f with
+  | Some f =>
+      abs_clear f t
+  | None => None
+  end.
+
+(* Axiom filter_empty : filter. *)
+
+Definition ok_until (f : filter) (t : Z) : Prop :=
+  match f with
+  | Some (mk_filter window_hi last_timestamp num_clears normal_frames) =>
+      0 <= t - last_timestamp <= Tc /\
+        last_timestamp < window_hi /\
+        (window_hi - 1 - last_timestamp) / Tc + num_clears >= num_slots
+  | None => False
+  end.
+
+Lemma query_clear : forall f t t' h b,
+  ok_until f t ->
+  filter_query f (t', h) = Some b ->
+  filter_query (filter_clear f t) (t', h) = Some b.
+Proof.
+  intros.
+Admitted.
+
+Lemma query_insert_same : forall f t t' h,
+  t <= t' < t+T ->
+  ok_until f t ->
   filter_query (filter_insert f (t, h)) (t', h) = Some true.
 Admitted.
 
-Lemma filter_query_insert_other : forall f t t' h h',
+Lemma query_insert_other : forall f t t' h h',
+  ok_until f t ->
   filter_query f (t', h') = Some true ->
   filter_query (filter_insert f (t, h)) (t', h') = Some true.
 Admitted.
 
-Lemma filter_query_empty : forall t h,
-  filter_query filter_empty (t, h) = Some false.
+Lemma ok_insert : forall f t t' h,
+  t <= t' <= t + Tc ->
+  ok_until f t ->
+  ok_until (filter_insert f (t, h)) t'.
 Admitted.
 
-Lemma isSome_filter_insert : forall f t h,
-  isSome f ->
-  isSome (filter_insert f (t, h)).
+Notation abs_refresh := (@filter_refresh header_type num_frames num_slots frame_time tick_time).
+
+Definition ok_until1 (f : filter) (new_timestamp : Z) (t : Z) : Prop :=
+  match f with
+  | Some (mk_filter window_hi _ num_clears normal_frames) =>
+      0 <= t - new_timestamp <= Tc /\
+        new_timestamp < window_hi /\
+        (window_hi - 1 - new_timestamp) / Tc + (num_clears + 1) >= num_slots
+  | None => False
+  end.
+
+Lemma ok_refresh : forall f t t',
+  t <= t' <= t + Tc ->
+  ok_until (Some f) t ->
+  ok_until1 (abs_refresh f t) t t'.
+Proof.
+  intros * H_t' H_ok_until.
+  destruct f as [window_hi last_timestamp num_clears normal_frames].
+  simpl in *.
+  replace (last_timestamp <=? t) with true by lia.
+  replace (t <=? last_timestamp + tick_time) with true by (pose Tc_le_tick_time; lia).
+  destruct (t >=? window_hi) eqn:?H.
+  - assert (0 <= window_hi - 1 - last_timestamp < Tc) by (pose Tc_le_tick_time; lia).
+    rewrite Z.div_small in H_ok_until by lia.
+    replace (num_clears >=? num_slots) with true by lia.
+    simpl.
+    split; only 1 : lia.
+    split; only 1 : (pose Tc_le_frame_time; lia).
+    pose Tc_mul_num_slots_ge_frame_time.
+    admit.
+  - simpl.
+    split; only 1 : lia.
+    split; only 1 : lia.
+    assert ((window_hi - 1 - last_timestamp + (-1) * Tc) / Tc <= (window_hi - 1 - t) / Tc). {
+      apply Z.div_le_mono. 2 : lia.
+      admit.
+    }
+    rewrite Zdiv.Z_div_plus in * by admit.
+    lia.
 Admitted.
 
-Lemma isSome_filter_clear_insert : forall f t t' h,
-  isSome (filter_clear f t') ->
-  isSome (filter_clear (filter_insert f (t, h)) t').
-Admitted.
+Lemma ok_clear : forall f t t',
+  t <= t' <= t + Tc ->
+  ok_until f t ->
+  ok_until (filter_clear f t) t'.
+Proof.
+  intros * H_t' H_ok_until.
+  destruct f. 2 : inv H_ok_until.
+  pose proof (H_ok_refresh := ok_refresh f t t' ltac:(auto) ltac:(auto)).
+  unfold filter_clear, abs_clear in *.
+  destruct (abs_refresh f t). 2 : inv H_ok_refresh.
+  destruct f0. apply H_ok_refresh.
+Qed.
 
-(* This is only true if we force f to be None as soon as Tc interval is voilated. *)
-Lemma isSome_filter_clear_clear : forall f t t',
-  0 <= t'-t < Tc ->
-  isSome (filter_clear f t) ->
-  isSome (filter_clear (filter_clear f t) t').
-Admitted.
-
-Lemma isSome_filter_clear_empty : forall t,
-  isSome (filter_clear filter_empty t).
-Admitted.
+(* Lemma ok_empty: forall t,
+  ok_until empty t. *)
 
 End LightFilter.
